theories/steps.v
@@ -24,3 +24,123 @@ Record state_wf' σ := {
 }.
 
 Instance state_wf : Wellformed state :=  state_wf'.
+
+(** Steps preserve wellformedness *)
+
+Lemma init_mem_foldr' l n h (m: nat):
+  init_mem (l +ₗ m) n h =
+  fold_right (λ (i: nat) hi, <[(l +ₗ i):=LitV ☠%V]> hi) h (seq m n).
+Proof.
+  revert l h m. induction n as [|n IHn]; intros l h m; [done|]. simpl. f_equal.
+  by rewrite shift_loc_assoc -(Nat2Z.inj_add m 1) Nat.add_1_r IHn.
+Qed.
+Lemma init_mem_foldr l n h:
+  init_mem l n h =
+  fold_right (λ (i: nat) hi, <[(l +ₗ i):=LitV ☠%V]> hi) h (seq 0 n).
+Proof. by rewrite -init_mem_foldr' shift_loc_0. Qed.
+
+Lemma free_mem_foldr' l n h (m: nat):
+  free_mem (l +ₗ m) n h =
+  fold_right (λ (i: nat) hi, delete (l +ₗ i) hi) h (seq m n).
+Proof.
+  revert l h m. induction n as [|n IHn]; intros l h m; [done|]. simpl. f_equal.
+  by rewrite shift_loc_assoc -(Nat2Z.inj_add m 1) Nat.add_1_r IHn.
+Qed.
+Lemma free_mem_foldr l n h:
+  free_mem l n h =
+  fold_right (λ (i: nat) hi, delete (l +ₗ i) hi) h (seq 0 n).
+Proof. by rewrite -free_mem_foldr' shift_loc_0. Qed.
+
+Lemma init_stacks_foldr' l n h si (m: nat):
+  init_stacks (l +ₗ m) n h si =
+  fold_right (λ (i: nat) hi, <[(l +ₗ i):=mkBorStack [si] None]> hi) h (seq m n).
+Proof.
+  revert l h m. induction n as [|n IHn]; intros l h m; [done|]. simpl. f_equal.
+  by rewrite shift_loc_assoc -(Nat2Z.inj_add m 1) Nat.add_1_r IHn.
+Qed.
+Lemma init_stacks_foldr l n h si:
+  init_stacks l n h si =
+  fold_right (λ (i: nat) hi, <[(l +ₗ i):=mkBorStack [si] None]> hi) h (seq 0 n).
+Proof. by rewrite -init_stacks_foldr' shift_loc_0. Qed.
+
+Lemma foldr_gmap_dom `{Countable K} {A B C: Type}
+  (ma: gmap K A) (mb: gmap K B) (a: A) (b: B) (cs: list C) (f: C → K):
+  dom (gset K) ma ≡ dom (gset K) mb →
+  dom (gset K) (foldr (λ (c: C) ma, <[f c := a]> ma) ma cs)
+  ≡ dom (gset K) (foldr (λ (c: C) mb, <[f c := b]> mb) mb cs).
+Proof.
+  intros. induction cs; simpl; [done|].
+  by rewrite 2!dom_insert IHcs.
+Qed.
+
+Lemma foldr_gmap_insert_lookup `{Countable K} {A C: Type}
+  (ma: gmap K A) (a ka: A) (cs: list C) (f: C → K) (k: K):
+  (foldr (λ (c: C) ma, <[f c := a]> ma) ma cs) !! k = Some ka →
+  ka = a ∨ ma !! k = Some ka.
+Proof.
+  induction cs as [|a' ? IHm]; simpl; [naive_solver|].
+  case (decide (f a' = k)) => [->|?].
+  - rewrite lookup_insert. naive_solver.
+  - by rewrite lookup_insert_ne.
+Qed.
+
+Lemma foldr_gmap_insert_lookup_neq `{Countable K} {A C: Type}
+  (ma: gmap K A) (a ka: A) (cs: list C) (f: C → K) (k: K) (NEq: ka ≠ a):
+  (foldr (λ (c: C) ma, <[f c := a]> ma) ma cs) !! k = Some ka →
+  ma !! k = Some ka.
+Proof.
+  intros Eq. by destruct (foldr_gmap_insert_lookup _ _ _ _ _ _ Eq).
+Qed.
+
+Lemma alloc_step_wf σ σ' e e' l bor T amod:
+  base_step e σ.(cheap) (Some $ AllocEvt l bor T amod) e' σ'.(cheap) [] →
+  instrumented_step σ.(cheap) σ.(cstk) σ.(cbar) σ.(cclk)
+                    (Some $ AllocEvt l bor T amod)
+                  σ'.(cheap) σ'.(cstk) σ'.(cbar) σ'.(cclk) →
+  Wf σ → Wf σ'.
+Proof.
+  destruct σ as [h stk bar clk].
+  destruct σ' as [h' stk' bar' clk']. simpl.
+  intros BS IS WF. inversion BS. clear BS. simplify_eq.
+  destruct (tsize T) eqn:Eqs.
+  - inversion IS; clear IS; simplify_eq; constructor; simpl.
+    + rewrite Eqs /=. apply WF.
+    + apply WF.
+    + rewrite Eqs /=. apply WF.
+    + rewrite Eqs /=. apply WF.
+    + rewrite Eqs /=. apply WF.
+    + move => ?? bor /(state_wf_mem_bor _ WF).
+      destruct bor as [|[]]; simpl; lia.
+    + rewrite Eqs /=.
+      move => ? stack /(state_wf_stack_frozen _ WF).
+      destruct (stack.(frozen_since)); simpl; lia.
+    + rewrite Eqs /=.
+      move => ?? si Eq In. move : (state_wf_stack_item _ WF _ _ _ Eq In).
+      destruct si; [simpl; lia|done..].
+  - inversion IS; clear IS; simplify_eq; constructor; cbn -[ init_mem].
+    + rewrite Eqs init_stacks_foldr init_mem_foldr. apply foldr_gmap_dom, WF.
+    + intros l1 l2 bor. rewrite init_mem_foldr.
+      intros [|Eq]%foldr_gmap_insert_lookup; [done|].
+      by apply (state_wf_mem_bor _ WF _ _ _ Eq).
+    + intros l1 stack. rewrite init_stacks_foldr.
+      intros [->|Eq]%foldr_gmap_insert_lookup; [done|].
+      by apply (state_wf_stack_frozen _ WF _ _ Eq).
+    + intros l1 stack si. rewrite init_stacks_foldr.
+      intros [->|Eq]%foldr_gmap_insert_lookup.
+      * by intros ->%elem_of_list_singleton.
+      * by apply (state_wf_stack_item _ WF _ _ _ Eq).
+    + rewrite Eqs init_stacks_foldr init_mem_foldr. apply foldr_gmap_dom, WF.
+    + intros l1 l2 bor. rewrite init_mem_foldr.
+      intros [|Eq]%foldr_gmap_insert_lookup; [done|].
+      move : (state_wf_mem_bor _ WF _ _ _ Eq).
+      destruct bor as [|[]]; simpl; lia.
+    + intros l1 stack. rewrite init_stacks_foldr.
+      intros [->|Eq]%foldr_gmap_insert_lookup; [done|].
+      move : (state_wf_stack_frozen _ WF _ _ Eq).
+      destruct stack.(frozen_since); simpl; lia.
+    + intros l1 stack si. rewrite init_stacks_foldr.
+      intros [->|Eq]%foldr_gmap_insert_lookup.
+      * intros ->%elem_of_list_singleton. lia.
+      * move => /(state_wf_stack_item _ WF _ _ _ Eq).
+        destruct si; [simpl; lia|done..].
+Qed.
